refocusing_machine.v
@@ -1,199 +1,15 @@
-Require Import Util.
+
+(*** Signatures ***)
+
+
 Require Import reduction_semantics.
-Require Export reduction_strategy.
 Require Import refocusing_semantics.
-Require Export abstract_machine.
-Require Export refocusing_machine_sig.
+Require Import abstract_machine.
 
 
 
-
-Module PreAbstractMachine (R : RED_LANG) (RS : RED_REF_SEM R) 
-           : PRE_ABSTRACT_MACHINE R RS.
-
-  Module ST := RS.ST.
-  Export ST.
-  Import R.
-
-
-  Inductive dec : term -> forall {k1 k2}, context k1 k2 -> decomp k1 -> Prop :=
-
-  | d_dec  : forall t {k1 k2} (c : context k1 k2) {r},
-               dec_term t k2 = in_red r -> 
-               dec t c (d_red r c)
-  | d_v    : forall t {k1 k2} {c : context k1 k2} {v d},
-               dec_term t k2 = in_val v ->
-               decctx v c d ->
-               dec t c d
-  | d_term : forall t {t0 k1 k2} {c : context k1 k2} {ec d},
-               dec_term t k2 = in_term t0 ec ->
-               dec t0 (ec=:c) d ->
-               dec t c d
-
-  with decctx : forall {k2}, value k2 -> 
-                    forall {k1}, context k1 k2 -> decomp k1 -> Prop :=
-
-  | dc_end  : forall {k} (v : value k), 
-                ~ dead_ckind k ->
-                decctx v [.] (d_val v)
-  | dc_dec  : forall ec {k2} (v : value (k2+>ec)) {k1} (c : context k1 k2) {r},
-                dec_context ec k2 v = in_red r ->
-                decctx v (ec=:c) (d_red r c)
-  | dc_val  : forall {k2} {v0 : value k2} ec (v : value (k2+>ec)) 
-                     {k1} {c  : context k1 k2} {d},
-                dec_context ec k2 v = in_val v0 ->
-                decctx v0 c d ->
-                decctx v (ec=:c) d
-  | dc_term : forall ec {ec0 k2} (v : value (k2+>ec)) 
-                            {k1} {c : context k1 k2} {t d},
-                dec_context ec k2 v = in_term t ec0 ->
-                dec t (ec0=:c) d ->
-                decctx v (ec=:c) d.
-
-  Scheme dec_Ind    := Induction for dec Sort Prop
-    with decctx_Ind := Induction for decctx Sort Prop.
-
-
-  Inductive iter : forall {k}, decomp k -> value k -> Prop :=
-  | i_val : forall {k} (v : value k), 
-              iter (d_val v) v
-  | i_red : forall {k2} (r : redex k2) {t k1} {c : context k1 k2} {d v},
-              contract r = Some t -> 
-              dec t c d -> 
-              iter d v ->
-              iter (d_red r c) v.
-
-
-  Inductive eval : term -> value init_ckind -> Prop :=
-  | e_intro : forall {t d v}, dec t [.] d -> iter d v -> eval t v.
-
-End PreAbstractMachine.
-
-
-
-
-Module StagedAbstractMachine (R : RED_LANG) (RS : RED_REF_SEM R) 
-           : STAGED_ABSTRACT_MACHINE R RS.
-
-  Module ST := RS.ST.
-  Import R.
-  Export ST.
-
-
-  Inductive dec : term -> forall {k1 k2}, context k1 k2 -> value k1 -> Prop :=
-
-  | d_dec  : forall t {k1 k2} {c : context k1 k2} {r v},
-               dec_term t k2 = in_red r -> 
-               iter (d_red r c) v ->
-               dec t c v
-  | d_v    : forall t {k1 k2} {c : context k1 k2} {v v0},
-               dec_term t k2 = in_val v -> 
-               decctx v c v0 ->
-               dec t c v0
-  | d_many : forall t {t0 ec k1 k2} {c : context k1 k2} {v},
-               dec_term t k2 = in_term t0 ec -> 
-               dec t0 (ec=:c) v ->
-               dec t c v
-
-  with decctx : forall {k2}, value k2 -> 
-                    forall {k1}, context k1 k2 -> value k1 -> Prop :=
-
-  | dc_end  : forall {k} {v v0 : value k},
-                ~ dead_ckind k ->
-                iter (d_val v) v0 ->
-                decctx v [.] v0
-  | dc_dec  : forall ec {k2} (v : value (k2+>ec)) {k1} {c : context k1 k2} {r v0},
-                dec_context ec k2 v = in_red r -> 
-                iter (d_red r c) v0 ->
-                decctx v (ec=:c) v0
-  | dc_val  : forall ec {k2} (v : value (k2+>ec)) {v0 k1} {c : context k1 k2} {v1},
-                dec_context ec k2 v = in_val v0 -> 
-                decctx v0 c v1 ->
-                decctx v (ec=:c) v1
-  | dc_term : forall ec {k2} (v : value (k2+>ec)) {t ec0 k1} {c : context k1 k2} {v0},
-                dec_context ec k2 v = in_term t ec0 -> 
-                dec t (ec0=:c) v0 ->
-                decctx v (ec=:c) v0
-
-  with iter : forall {k}, decomp k -> value k -> Prop :=
-
-  | i_val : forall {k} (v : value k), 
-              iter (d_val v) v
-  | i_red : forall {k2} (r : redex k2) {k1} {c : context k1 k2} {t v},
-              contract r = Some t -> 
-              dec t c v -> 
-              iter (d_red r c) v.
-
-  Scheme dec_Ind    := Induction for dec    Sort Prop
-    with decctx_Ind := Induction for decctx Sort Prop
-    with iter_Ind   := Induction for iter   Sort Prop.
-
-
-  Inductive eval : term -> value init_ckind -> Prop :=
-  | e_intro : forall {t v}, dec t [.] v -> eval t v.
-
-End StagedAbstractMachine.
-
-
-
-
-Module EvalApplyMachine (R : RED_LANG) (RS : RED_REF_SEM R)
-           : EVAL_APPLY_MACHINE R RS.
-
-  Module ST := RS.ST.
-  Export ST.
-  Import R.
-
-
-  Inductive dec : term -> forall {k1 k2}, context k1 k2 -> value k1 -> Prop :=
-
-  | d_d_r  : forall t {t0 k1 k2} {c : context k1 k2} {r : redex k2} {v},
-               dec_term t k2 = in_red r -> 
-               contract r = Some t0 -> 
-               dec t0 c v ->
-               dec t c v
-  | d_v    : forall t {k1 k2} {c : context k1 k2} {v v0},
-               dec_term t k2 = in_val v -> 
-               decctx v c v0 ->
-               dec t c v0
-  | d_term : forall t {t0 ec k1 k2} {c : context k1 k2} {v},
-               dec_term t k2 = in_term t0 ec -> 
-               dec t0 (ec=:c) v ->
-               dec t c v
-
-  with decctx : forall {k2}, value k2 -> 
-                    forall {k1}, context k1 k2 -> value k1 -> Prop :=
-
-  | dc_end : forall {k} (v : value k), 
-               ~ dead_ckind k ->
-               decctx v [.] v
-  | dc_red : forall ec {k2} (v : value (k2+>ec)) {k1} {c : context k1 k2} {r t v0},
-               dec_context ec k2 v = in_red r -> 
-               contract r = Some t -> 
-               dec t c v0 ->
-               decctx v (ec=:c) v0
-  | dc_rec : forall ec {k2} (v : value (k2+>ec)) {k1} {c : context k1 k2} {v0 v1},
-               dec_context ec k2 v = in_val v0 -> 
-               decctx v0 c v1 ->
-               decctx v (ec=:c) v1
-  | dc_trm : forall ec {k2} (v : value (k2+>ec)) {k1} {c : context k1 k2} {t ec0 v0},
-               dec_context ec k2 v = in_term t ec0 -> 
-               dec t (ec0=:c) v0 ->
-               decctx v (ec=:c) v0.
-
-  Scheme dec_Ind    := Induction for dec    Sort Prop
-    with decctx_Ind := Induction for decctx Sort Prop.
-
-
-  Inductive eval : term -> value init_ckind -> Prop :=
-  | e_intro : forall {t v}, dec t [.] v -> eval t v.
-
-End EvalApplyMachine.
-
-
-
-
-Module ProperEAMachine (R : RED_LANG) (RS : RED_REF_SEM R) <: ABSTRACT_MACHINE.
+Module Type REF_EVAL_APPLY_MACHINE (R : RED_LANG) (RS : RED_REF_SEM R) 
+                                                    <: DET_ABSTRACT_MACHINE.
 
   Import R.
   Import RS.ST.
@@ -209,9 +25,21 @@ Module ProperEAMachine (R : RED_LANG) (RS : RED_REF_SEM R) <: ABSTRACT_MACHINE.
 
   Definition c_init t            := c_eval t [.](init_ckind).
   Definition c_final (v : value) := c_apply [.] v.
+  (*Definition final_of (st : configuration) : option value := 
+      match st with 
+      | c_apply k _ [.] v => 
+          match is_initial k with
+          | left H => match H in _ = k return R.value k -> option value with
+                      | eq_refl => fun v => Some v
+                      end v
+          | _      => None
+          end
+      | _ => None
+      end.
+  Axiom final_of_correct : forall c v, final_of c = Some v <-> c_final v = c.*)
 
 
-  Reserved Notation "c1 → c2" (at level 40, no associativity).
+  Reserved Notation "st1 → st2" (at level 40, no associativity).
 
   Inductive trans : configuration -> configuration -> Prop :=
 
@@ -234,16 +62,12 @@ Module ProperEAMachine (R : RED_LANG) (RS : RED_REF_SEM R) <: ABSTRACT_MACHINE.
                dec_context ec k2 v = in_term t ec0 ->
                c_apply (ec=:c) v → c_eval t (ec0=:c)
 
-  where "c1 → c2" := (trans c1 c2).
+  where "st1 → st2" := (trans st1 st2).
   Definition transition := trans.
   Hint Unfold transition.
 
+  Axiom final_correct : forall v st, ~ c_final v → st.
 
-  Lemma final_correct : forall v st, ~ c_final v → st.
-
-  Proof.
-    inversion 1.
-  Qed.
 
 
   Reserved Notation "c1 →+ c2" (at level 40, no associativity).
@@ -283,12 +107,228 @@ Module ProperEAMachine (R : RED_LANG) (RS : RED_REF_SEM R) <: ABSTRACT_MACHINE.
       end.
 
 
-  Lemma next_correct  : forall c1 c2, next_conf c1 = Some c2 <-> c1 → c2.
+  Axiom next_correct  : forall c1 c2, next_conf c1 = Some c2 <-> c1 → c2.
+
+End REF_EVAL_APPLY_MACHINE.
+
+
+
+
+
+Module Type REF_PUSH_ENTER_MACHINE (R : RED_LANG) (PERS : PE_RED_REF_SEM R) 
+                                                       <: DET_ABSTRACT_MACHINE.
+
+  Import R.
+  Import PERS.ST.
+
+
+  Definition term  := term.
+  Definition value := value init_ckind.
+
+
+  Inductive conf : Set :=
+  | c_eval  : term -> forall {k1 k2}, context k1 k2 -> conf
+  | c_fin : forall {k}, R.value k                -> conf.
+  Definition configuration := conf.
+
+  Definition c_init t  := c_eval t [.](init_ckind).
+  Definition c_final (v : value) := c_fin v.
+  (*Definition final_of (st : configuration) : option value := 
+      match st with 
+      | c_fin k v => 
+          match is_initial k with
+          | left H => match H in _ = k return R.value k -> option value with
+                      | eq_refl => fun v => Some v
+                      end v
+          | _      => None
+          end
+      | _ => None
+      end.
+  Axiom final_of_correct : forall c v, final_of c = Some v <-> c_final v = c.*)
+
+
+  Reserved Notation "c1 → c2" (at level 40, no associativity).
+
+  Inductive trans : configuration -> configuration -> Prop :=
+
+  | t_red  : forall t {k1 k2} (c : context k1 k2) {t0 r},
+               dec_term t k2 = in_red r -> 
+               contract r = Some t0 ->
+               c_eval t c → c_eval t0 c
+  | t_cval : forall t {k} {v : R.value k},
+               dec_term t k = in_val v ->
+               c_eval t [.](k) → c_fin v
+  | t_cred : forall t ec {t0} {k1 k2} (c : context k1 k2) {v r},
+               dec_term t (k2+>ec) = in_val v ->
+               dec_context ec k2 v = in_red r ->
+               contract r = Some t0 ->
+               c_eval t (ec=:c) → c_eval t0 c
+  | t_crec : forall t ec {t0 ec0 k1 k2} (c : context k1 k2) {v},
+               dec_term t (k2+>ec) = in_val v ->
+               dec_context ec k2 v = in_term t0 ec0 ->
+               c_eval t (ec=:c) → c_eval t0 (ec0=:c)
+  | t_rec  : forall t {t0 ec k1 k2} (c : context k1 k2),
+               dec_term t k2 = in_term t0 ec ->
+               c_eval t c → c_eval t0 (ec=:c)
+
+  where "c1 → c2" := (trans c1 c2).
+  Definition transition := trans.
+  Hint Unfold transition.
+
+  Axiom final_correct : forall v st, ~ c_final v → st.
+
+
+  Reserved Notation "c1 →+ c2" (at level 40, no associativity).
+  Reserved Notation "c1 →* c2" (at level 40, no associativity).
+
+  Inductive trans_close : configuration -> configuration -> Prop :=
+  | one_step   : forall c1 c2,     c1 → c2  ->  c1 →+ c2
+  | multi_step : forall c1 c2 c3,  c1 → c2  ->  c2 →+ c3  ->  c1 →+ c3
+  where "c1 →+ c2" := (trans_close c1 c2).
+
+  Definition trans_ref_close c1 c2 := c1 = c2 \/ trans_close c1 c2.
+  Notation "c1 →* c2" := (trans_ref_close c1 c2).
+
+  Inductive eval : term -> value -> Prop :=
+  | e_intro : forall t v, trans_close (c_init t) (c_final v) -> eval t v.
+
+
+  Definition next_conf st :=
+      match st with
+      | c_eval t _ k2 c  => 
+            match dec_term t k2 with
+            | in_red r => option_map (fun t' => c_eval t' c) (contract r)
+            | in_val v => match c in context _ k2 
+                              return R.value k2 -> option configuration with 
+                          | [.]          => fun _ => Some (c_fin v)
+                          | ccons ec k c => fun v => 
+                                match dec_context ec k v with
+                                | in_red r       => option_map (fun t' => c_eval t' c)
+                                                               (contract r)
+                                | in_term t' ec' => Some (c_eval t' (ec'=:c))
+                                | _              => None
+                                end
+                          end v
+            | in_term t ec => Some (c_eval t (ec=:c))
+            | in_dead => None
+            end
+      | _ => None
+      end.
+
+
+  Axiom next_correct  : forall c1 c2, next_conf c1 = Some c2 <-> c1 → c2.
+
+End REF_PUSH_ENTER_MACHINE.
+
+
+
+
+
+(*** Functors ***)
+
+
+Require Import Util.
+Require Export reduction_strategy.
+
+
+
+
+Module RefEvalApplyMachine (R : RED_LANG) (RS : RED_REF_SEM R) 
+                                                 <: REF_EVAL_APPLY_MACHINE R RS.
+
+  Import R.
+  Import RS.ST.
+
+
+  Definition term  := term.
+  Definition value := value init_ckind.
+
+  Inductive conf : Set :=
+  | c_eval  : term -> forall {k1 k2}, context k1 k2 -> conf
+  | c_apply : forall {k1 k2}, context k1 k2 -> R.value k2 -> conf.
+  Definition configuration := conf.
+
+  Definition c_init t            := c_eval t [.](init_ckind).
+  Definition c_final (v : value) := c_apply [.] v.
+
+
+  Reserved Notation "c1 → c2" (at level 40, no associativity).
+
+  Inductive trans : configuration -> configuration -> Prop :=
+
+  | t_red  : forall t {k1 k2} (c : context k1 k2) {r : redex k2} {t0},
+               dec_term t k2 = in_red r -> contract r = Some t0 ->
+               c_eval t c → c_eval t0 c
+  | t_val  : forall t {k1 k2} (c : context k1 k2) {v},
+      	       dec_term t k2 = in_val v ->
+               c_eval t c → c_apply c v
+  | t_term : forall t {k1 k2} (c : context k1 k2) {t0 ec},
+               dec_term t k2 = in_term t0 ec ->
+               c_eval t c → c_eval t0 (ec=:c)
+  | t_cred : forall ec {k2} (v : R.value (k2+>ec)) {k1} (c : context k1 k2) {r t},
+               dec_context ec k2 v = in_red r -> contract r = Some t ->
+               c_apply (ec=:c) v → c_eval t c
+  | t_cval : forall ec {k2} (v : R.value (k2+>ec)) {k1} (c : context k1 k2) {v0},
+               dec_context ec k2 v = in_val v0 ->
+               c_apply (ec=:c) v → c_apply c v0
+  | t_cterm: forall ec {k2} (v : R.value (k2+>ec)) {k1} (c : context k1 k2) {t ec0},
+               dec_context ec k2 v = in_term t ec0 ->
+               c_apply (ec=:c) v → c_eval t (ec0=:c)
+
+  where "c1 → c2" := (trans c1 c2).
+  Definition transition := trans.
+  Hint Unfold transition.
+
+
+  Lemma final_correct : forall v st, ~ c_final v → st.
+
+  Proof. inversion 1. Qed.
+
+
+  Reserved Notation "c1 →+ c2" (at level 40, no associativity).
+  Reserved Notation "c1 →* c2" (at level 40, no associativity).
+
+  Inductive trans_close : configuration -> configuration -> Prop :=
+  | one_step   : forall c1 c2,     c1 → c2  ->  c1 →+ c2
+  | multi_step : forall c1 c2 c3,  c1 → c2  ->  c2 →+ c3  ->  c1 →+ c3
+  where "c1 →+ c2" := (trans_close c1 c2).
+
+  Definition trans_ref_close c1 c2 := c1 = c2 \/ trans_close c1 c2.
+  Notation "c1 →* c2" := (trans_ref_close c1 c2).
+
+
+  Inductive eval : term -> value -> Prop :=
+  | e_intro : forall t v, trans_close (c_init t) (c_final v) -> eval t v.
+
+
+  Definition next_conf st :=
+      match st with
+      | c_eval t _ k2 c  => 
+            match dec_term t k2 with
+            | in_red r => option_map (fun t' => c_eval t' c) (contract r)
+            | in_val v => Some (c_apply c v)
+            | in_term t ec => Some (c_eval t (ec=:c))
+            | in_dead => None
+            end
+      | c_apply _ _ (ccons ec k c) v => 
+            match dec_context ec k v with
+            | in_red r => option_map (fun t' => c_eval t' c) (contract r)
+            | in_val v => Some (c_apply c v)
+            | in_term t ec => Some (c_eval t (ec=:c))
+            | in_dead => None
+            end
+      | c_apply _ _ [.] v => 
+            None
+      end.
+
+
+
+  Lemma next_correct : forall c1 c2, next_conf c1 = Some c2 <-> c1 → c2.
 
   Proof.
-  intros c1 c2; split; intro H.
+    intros c1 c2; split; intro H.
 
-  {
+  (* -> *) {
       destruct c1; simpl in H.
       - remember (dec_term t k2) as dc.
         destruct dc.
@@ -317,7 +357,7 @@ Module ProperEAMachine (R : RED_LANG) (RS : RED_REF_SEM R) <: ABSTRACT_MACHINE.
         + inversion H.
   }
 
-  {
+  (* <- *) {
       destruct H;
           simpl;
           match goal with H : @eq (interm_dec _) _ _ |- _ => rewrite H end;
@@ -327,62 +367,13 @@ Module ProperEAMachine (R : RED_LANG) (RS : RED_REF_SEM R) <: ABSTRACT_MACHINE.
   }
   Qed.
 
-End ProperEAMachine.
+End RefEvalApplyMachine.
 
 
 
 
-Module PushEnterMachine (R : RED_LANG) (PERS : PE_RED_REF_SEM R)
-           : PUSH_ENTER_MACHINE R PERS.
-
-  Module ST := PERS.ST.
-  Export ST.
-  Import R.
-
-
-  Axiom dec_context_not_val : 
-      forall ec {k} v1 v0, dec_context ec k v0 <> in_val v1.
-
-  Axiom dec_term_value : 
-      forall {k} (v : value k), dec_term v k = in_val v.
-
-
-  Inductive dec : term -> forall {k1 k2}, context k1 k2 -> value k1 -> Prop :=
-
-  | dec_r    : forall t {t0 k1 k2} {c : context k1 k2} {r  v},
-                 dec_term t k2 = in_red r -> 
-                 contract r = Some t0 -> 
-                 dec t0 c v ->
-                 dec t c v
-  | dec_val  : forall t {k} {v : value k},
-                 dec_term t k = in_val v ->
-                 dec t [.] v
-  | dec_v_t  : forall t ec {t0 ec0} {k1 k2} {c : context k1 k2} {v v0},
-                 dec_term t (k2+>ec) = in_val v -> 
-                 dec_context ec k2 v = in_term t0 ec0 -> 
-                 dec t0 (ec0=:c) v0 ->
-                 dec t (ec=:c) v0
-  | dec_red  : forall t ec {t0} {k1 k2} {c : context k1 k2} {v v0 r},
-                 dec_term t (k2+>ec) = in_val v ->
-                 dec_context ec k2 v = in_red r -> 
-                 contract r = Some t0 -> 
-                 dec t0 c v0 ->
-                 dec t (ec=:c) v0
-  | dec_rec  : forall t {t0 ec} {k1 k2} {c : context k1 k2} {v},
-                 dec_term t k2 = in_term t0 ec ->
-                 dec t0 (ec=:c) v ->
-                 dec t c v.
-
-
-  Inductive eval : term -> value init_ckind -> Prop :=
-  | e_intro : forall {t v}, dec t [.] v -> eval t v.
-
-End PushEnterMachine.
-
-
-
-
-Module ProperPEMachine (R : RED_LANG) (PERS : PE_RED_REF_SEM R) <: ABSTRACT_MACHINE.
+Module RefPushEnterMachine (R : RED_LANG) (PERS : PE_RED_REF_SEM R) 
+                                                 <: REF_PUSH_ENTER_MACHINE R PERS.
 
   Import R.
   Import PERS.ST.
@@ -431,10 +422,7 @@ Module ProperPEMachine (R : RED_LANG) (PERS : PE_RED_REF_SEM R) <: ABSTRACT_MACH
 
 
   Lemma final_correct : forall v st, ~ c_final v → st.
-
-  Proof.
-    inversion 1.
-  Qed.
+  Proof. inversion 1. Qed.
 
 
   Reserved Notation "c1 →+ c2" (at level 40, no associativity).
@@ -479,9 +467,9 @@ Module ProperPEMachine (R : RED_LANG) (PERS : PE_RED_REF_SEM R) <: ABSTRACT_MACH
   Lemma next_correct  : forall c1 c2, next_conf c1 = Some c2 <-> c1 → c2.
 
   Proof.
-  intros c1 c2; split; intro H.
+    intros c1 c2; split; intro H.
 
-  {
+  (* -> *) {
       destruct c1; simpl in H.
       - remember (dec_term t k2) as dc.
         destruct dc.
@@ -507,7 +495,7 @@ Module ProperPEMachine (R : RED_LANG) (PERS : PE_RED_REF_SEM R) <: ABSTRACT_MACH
       - inversion H. 
   }
 
-  {
+  (* <- *) {
       destruct H;
           simpl;
           match goal with H : @eq (interm_dec _) _ _ |- _ => rewrite H end;
@@ -517,4 +505,4 @@ Module ProperPEMachine (R : RED_LANG) (PERS : PE_RED_REF_SEM R) <: ABSTRACT_MACH
   }
   Qed.
 
-End ProperPEMachine.
+End RefPushEnterMachine.
