refocusing_machine_facts.v
@@ -1,0 +1,230 @@
+Require Import Util.
+Require Import Program.
+Require Import refocusing_semantics.
+Require Import refocusing_natural_semantics.
+Require Import refocusing_machine.
+Require Import reduction_semantics_facts.
+Require Import refocusing_semantics_facts.
+Require Import refocusing_natural_semantics_facts.
+
+
+
+
+Module RefEvalApplyMachine_Facts (R : RED_LANG) (RS : RED_REF_SEM R) 
+                                        (EAM : REF_EVAL_APPLY_MACHINE R RS).
+
+  Module RNS  := RefNaturalSem R RS.
+  Module RNSF := RefNaturalSem_Facts R RS RNS.
+  Import R.
+  Import RS.ST.
+  Import EAM.
+
+
+  Local Hint Constructors EAM.trans EAM.trans_close.
+  Local Hint Constructors RNS.dec RNS.decctx.
+
+
+  Lemma dec_RNS_eqv_EAM : forall {t k1 k2} (c : context k1 k2) {v}, 
+                              RNS.dec t c v <-> c_eval t c →+ c_apply [.] v.
+  Proof with eauto.
+    intros t k1 k2 c v; split; intro H.
+
+  (* -> *) {
+    induction H using RNS.dec_Ind with
+    (P := fun t _ _ c v  (_ : RNS.dec t c v) => 
+              c_eval t c  →+ c_apply [.] v)
+    (P0:= fun k2 v k1 c v' (_ : RNS.decctx v c v') => 
+              c_apply c v →+ c_apply [.] v' \/ k1 = k2 /\ [.](k1) ~= c /\ v ~=v');
+
+    intuition; dep_subst...
+  }
+
+  (* <- *) {
+    revert t k2 c H.
+
+    cut (forall st, st →+ c_apply [.] v -> 
+         match st with 
+         | c_eval t k1' _ c   => k1 = k1' -> forall v', v ~= v' -> RNS.dec t c v'
+         | c_apply k1' _ c v0 => k1 = k1' -> forall v', v ~= v' -> RNS.decctx v0 c v'
+         end).
+    { intros H t k2 c H0; apply (H _ H0)... }
+
+    intros st H.
+
+    dependent induction H;
+        match goal with H : _ → _ |- _ => 
+              dependent_destruction2 H end;
+        match goal with 
+        | H : dec_term _ ?k = _ |- _=> 
+              assert (~ dead_ckind k);
+              [ intro; rewrite dec_term_from_dead in H; solve[eauto] 
+              | ]
+        | H : dec_context _ ?k _ = _ |- _=> 
+              assert (~ dead_ckind k);
+              [ intro; rewrite dec_context_from_dead in H; 
+                solve [eauto using death_propagation] 
+              | ]
+        end;
+
+    intros; dep_subst...
+  }
+  Qed.
+
+
+
+  Lemma decctx_RNS_eqv_EAM : 
+      forall {k1 k2} (c : context k1 k2) {v0 v1}, 
+          RNS.decctx v0 c v1 <-> c_apply c v0 →+ c_apply [.] v1 \/
+                                 c_apply c v0 = c_apply [.] v1 /\ ~dead_ckind k1.
+
+  Proof with eauto.
+    intros k1 k2 c v0 v1; split; intro H.
+
+  (* -> *) {
+    induction H using RNS.decctx_Ind with
+    (P := fun t _ _ c v  (_ : RNS.dec t c v)     => 
+              c_eval t c  →+ c_apply [.] v)
+    (P0:= fun k2 v k1 c v' (_ : RNS.decctx v c v') => 
+              c_apply c v →+ c_apply [.] v' \/ 
+              c_apply c v = c_apply [.] v' /\ ~dead_ckind k1);
+
+    solve
+    [ intuition; dep_subst; eauto
+    | destruct IHdecctx as [H0 | [H0 H1]]; inversion H0; dep_subst; eauto ].
+
+  }
+
+  (* <- *) {
+    revert k2 v0 c H.
+
+    cut (forall st, st →+ c_apply [.] v1 -> 
+         match st with 
+         | c_eval t k1' _ c   => k1 = k1' -> forall v', v1 ~= v' -> RNS.dec t c v'
+         | c_apply k1' _ c v0 => k1 = k1' -> forall v', v1 ~= v' -> RNS.decctx v0 c v'
+         end).
+    { intros H t k2 c H0.
+      destruct H0 as [H0 | [H0 H1]]. 
+      - apply (H _ H0)...
+      - inversion H0; dep_subst... }
+
+    intros st H.
+    dependent induction H;
+        match goal with H : _ → _ |- _ => 
+              dependent_destruction2 H end;
+        match goal with 
+        | H : dec_term _ ?k = _ |- _=> 
+              assert (~ dead_ckind k);
+              [ intro; rewrite dec_term_from_dead in H; solve[eauto] 
+              | ]
+        | H : dec_context _ ?k _ = _ |- _=> 
+              assert (~ dead_ckind k);
+              [ intro; rewrite dec_context_from_dead in H; 
+                solve [eauto using death_propagation] 
+              | ]
+        end;
+
+    intros; dep_subst...
+  }
+  Qed.
+
+
+
+  Lemma eval_RNS_eqv_EAM : forall {t v}, RNS.eval t v <-> EAM.eval t v.
+  Proof.
+    intros t v; split; intro H;
+    solve 
+    [ dependent destruction H; constructor; apply dec_RNS_eqv_EAM; eauto ].
+  Qed.
+
+
+
+  Theorem dec_iter_composition :
+      forall {t k1 k2} {c : context k1 k2} {v},
+          (exists d, RS.dec t c d /\ RS.iter d v) <-> c_eval t c →+ c_apply [.] v.
+
+  Proof.
+    etransitivity; eauto using dec_RNS_eqv_EAM, RNSF.dec_iter_composition.
+  Qed.
+
+
+
+  Theorem decctx_iter_composition : forall {k1 k2} {c : context k1 k2} {v0 v1},
+
+          (exists d, RS.decctx v0 c d /\ RS.iter d v1) <-> 
+
+          c_apply c v0 →+ c_apply [.] v1 \/
+          c_apply c v0 = c_apply [.] v1 /\ ~dead_ckind k1.
+
+  Proof.
+    etransitivity; eauto using decctx_RNS_eqv_EAM, RNSF.decctx_iter_composition.
+  Qed.
+
+
+
+  Theorem eval_preservation : forall {t v}, RS.eval t v <-> EAM.eval t v.
+
+  Proof. etransitivity; eauto using RNSF.eval_preserved, eval_RNS_eqv_EAM. Qed.
+
+End RefEvalApplyMachine_Facts.
+
+
+
+
+Module PushEnterMachine_Facts (R : RED_LANG) (PERS : PE_RED_REF_SEM R) 
+                                        (PEM : REF_PUSH_ENTER_MACHINE R PERS).
+
+  Module PENS  := PE_RefNaturalSem R PERS.
+  Module PENSF := PE_RefNaturalSem_Facts R PERS PENS.
+  Import R PERS.ST.
+  Import PEM.
+
+
+
+  Local Hint Constructors PEM.trans PEM.trans_close PENS.dec.
+
+
+  Lemma dec_PENS_eqv_PEM : forall {t} {k1 k2} {c : context k1 k2} {v}, 
+                           PENS.dec t c v <-> c_eval t c →+ c_fin v.
+  Proof with eauto.
+    intros t k1 k2 v; split; intro H.
+
+  (* -> *) {
+    induction H...
+  }
+
+  (* <- *) {
+    dependent induction H;
+        match goal with H : _ → _ |- _ => 
+            dependent_destruction2 H end;
+    solve 
+    [ eauto
+    | inversion H0 as [? ? H | ? ? ? H ]; inversion H
+    | constructor; auto;
+      intro H; 
+      assert (H0 := dec_term_from_dead t _ H); rewrite H0 in *; 
+      discriminate ].
+  }
+  Qed.
+
+
+  Lemma eval_PENS_eqv_PEM : forall {t v}, PENS.eval t v <-> PEM.eval t v.
+  Proof.
+    intros t v; split; intro H;
+    solve
+    [ dependent destruction H; constructor; apply dec_PENS_eqv_PEM; eauto ].
+  Qed.
+
+
+  Theorem dec_iter_composition :
+      forall {t k1 k2} {c : context k1 k2} {v},
+          (exists d, PERS.dec t c d /\ PERS.iter d v) <-> c_eval t c →+ c_fin v.
+  Proof.
+    etransitivity; eauto using PENSF.dec_iter_composition, dec_PENS_eqv_PEM.
+  Qed.
+
+
+  Theorem eval_preserved : forall {t v}, PERS.eval t v <-> PEM.eval t v.
+
+  Proof. etransitivity; eauto using PENSF.eval_preserved, eval_PENS_eqv_PEM. Qed.
+
+End PushEnterMachine_Facts.
