refocusing_natural_semantics.v
@@ -1,0 +1,486 @@
+
+(*** Signatures ***)
+
+
+Require Import reduction_semantics.
+Require Import refocusing_semantics.
+
+
+
+
+Module Type PRE_REF_NATURAL_SEM (R : RED_LANG) (RS : RED_REF_SEM R).
+
+  Module ST := RS.ST.
+  Export ST.
+  Import R.
+
+
+  Inductive dec : term -> forall {k1 k2}, context k1 k2 -> decomp k1 -> Prop :=
+
+  | d_dec  : forall t {k1 k2} (c : context k1 k2) {r},
+               dec_term t k2 = in_red r -> 
+               dec t c (d_red r c)
+  | d_v    : forall t {k1 k2} {c : context k1 k2} {v d},
+               dec_term t k2 = in_val v ->
+               decctx v c d ->
+               dec t c d
+  | d_term : forall t {t0 k1 k2} {c : context k1 k2} {ec d},
+               dec_term t k2 = in_term t0 ec ->
+               dec t0 (ec=:c) d ->
+               dec t c d
+
+  with decctx : forall {k2}, value k2 -> 
+                    forall {k1}, context k1 k2 -> decomp k1 -> Prop :=
+
+  | dc_end  : forall {k} (v : value k), 
+                ~ dead_ckind k ->
+                decctx v [.] (d_val v)
+  | dc_dec  : forall ec {k2} (v : value (k2+>ec)) {k1} (c : context k1 k2) {r},
+                dec_context ec k2 v = in_red r ->
+                decctx v (ec=:c) (d_red r c)
+  | dc_val  : forall {k2} {v0 : value k2} ec (v : value (k2+>ec)) 
+                     {k1} {c  : context k1 k2} {d},
+                dec_context ec k2 v = in_val v0 ->
+                decctx v0 c d ->
+                decctx v (ec=:c) d
+  | dc_term : forall ec {ec0 k2} (v : value (k2+>ec)) 
+                            {k1} {c : context k1 k2} {t d},
+                dec_context ec k2 v = in_term t ec0 ->
+                dec t (ec0=:c) d ->
+                decctx v (ec=:c) d.
+
+  Scheme dec_Ind    := Induction for dec Sort Prop
+    with decctx_Ind := Induction for decctx Sort Prop.
+
+
+  Inductive iter : forall {k}, decomp k -> value k -> Prop :=
+  | i_val : forall {k} (v : value k), 
+              iter (d_val v) v
+  | i_red : forall {k2} (r : redex k2) {t k1} {c : context k1 k2} {d v},
+              contract r = Some t  ->  dec t c d  ->  iter d v ->
+              iter (d_red r c) v.
+
+
+  Inductive eval : term -> value init_ckind -> Prop :=
+  | e_intro : forall {t d v}, dec t [.] d -> iter d v -> eval t v.
+
+End PRE_REF_NATURAL_SEM.
+
+
+
+
+
+Module Type STAGED_REF_NATURAL_SEM (R : RED_LANG) (RS : RED_REF_SEM R).
+
+  Module ST := RS.ST.
+  Import R.
+  Export ST.
+
+
+  Inductive dec : term -> forall {k1 k2}, context k1 k2 -> value k1 -> Prop :=
+
+  | d_dec  : forall t {k1 k2} {c : context k1 k2} {r v},
+               dec_term t k2 = in_red r -> 
+               iter (d_red r c) v ->
+               dec t c v
+  | d_v    : forall t {k1 k2} {c : context k1 k2} {v v0},
+               dec_term t k2 = in_val v -> 
+               decctx v c v0 ->
+               dec t c v0
+  | d_many : forall t {t0 ec k1 k2} {c : context k1 k2} {v},
+               dec_term t k2 = in_term t0 ec -> 
+               dec t0 (ec=:c) v ->
+               dec t c v
+
+  with decctx : forall {k2}, value k2 -> 
+                    forall {k1}, context k1 k2 -> value k1 -> Prop :=
+
+  | dc_end  : forall {k} {v v0 : value k},
+                ~ dead_ckind k ->
+                iter (d_val v) v0 ->
+                decctx v [.] v0
+  | dc_dec  : forall ec {k2} (v : value (k2+>ec)) {k1} {c : context k1 k2} {r v0},
+                dec_context ec k2 v = in_red r -> 
+                iter (d_red r c) v0 ->
+                decctx v (ec=:c) v0
+  | dc_val  : forall ec {k2} (v : value (k2+>ec)) {v0 k1} {c : context k1 k2} {v1},
+                dec_context ec k2 v = in_val v0 -> 
+                decctx v0 c v1 ->
+                decctx v (ec=:c) v1
+  | dc_term : forall ec {k2} (v : value (k2+>ec)) {t ec0 k1} {c : context k1 k2} {v0},
+                dec_context ec k2 v = in_term t ec0 -> 
+                dec t (ec0=:c) v0 ->
+                decctx v (ec=:c) v0
+
+  with iter : forall {k}, decomp k -> value k -> Prop :=
+
+  | i_val : forall {k} (v : value k), 
+              iter (d_val v) v
+  | i_red : forall {k2} (r : redex k2) {k1} {c : context k1 k2} {t v},
+              contract r = Some t -> 
+              dec t c v -> 
+              iter (d_red r c) v.
+
+  Scheme dec_Ind    := Induction for dec Sort Prop
+    with decctx_Ind := Induction for decctx Sort Prop
+    with iter_Ind   := Induction for iter Sort Prop.
+
+
+  Inductive eval : term -> value init_ckind -> Prop :=
+  | e_intro : forall {t v}, dec t [.] v -> eval t v.
+
+End STAGED_REF_NATURAL_SEM.
+
+
+
+
+
+Module Type REF_NATURAL_SEM (R : RED_LANG) (RS : RED_REF_SEM R).
+
+  Module ST := RS.ST.
+  Export ST.
+  Import R.
+
+
+  Inductive dec : term -> forall {k1 k2}, context k1 k2 -> value k1 -> Prop :=
+
+  | d_d_r  : forall t {t0 k1 k2} {c : context k1 k2} {r : redex k2} {v},
+               dec_term t k2 = in_red r -> 
+               contract r = Some t0 -> 
+               dec t0 c v ->
+               dec t c v
+  | d_v    : forall t {k1 k2} {c : context k1 k2} {v v0},
+               dec_term t k2 = in_val v -> 
+               decctx v c v0 ->
+               dec t c v0
+  | d_term : forall t {t0 ec k1 k2} {c : context k1 k2} {v},
+               dec_term t k2 = in_term t0 ec -> 
+               dec t0 (ec=:c) v ->
+               dec t c v
+
+  with decctx : forall {k2}, value k2 -> 
+                    forall {k1}, context k1 k2 -> value k1 -> Prop :=
+
+  | dc_end : forall {k} (v : value k), 
+               ~ dead_ckind k ->
+               decctx v [.] v
+  | dc_red : forall ec {k2} (v : value (k2+>ec)) {k1} {c : context k1 k2} {r t v0},
+               dec_context ec k2 v = in_red r -> 
+               contract r = Some t -> 
+               dec t c v0 ->
+               decctx v (ec=:c) v0
+  | dc_rec : forall ec {k2} (v : value (k2+>ec)) {k1} {c : context k1 k2} {v0 v1},
+               dec_context ec k2 v = in_val v0 -> 
+               decctx v0 c v1 ->
+               decctx v (ec=:c) v1
+  | dc_trm : forall ec {k2} (v : value (k2+>ec)) {k1} {c : context k1 k2} {t ec0 v0},
+               dec_context ec k2 v = in_term t ec0 -> 
+               dec t (ec0=:c) v0 ->
+               decctx v (ec=:c) v0.
+
+  Scheme dec_Ind    := Induction for dec Sort Prop
+    with decctx_Ind := Induction for decctx Sort Prop.
+
+
+  Inductive eval : term -> value init_ckind -> Prop :=
+  | e_intro : forall {t v}, dec t [.] v -> eval t v.
+
+End REF_NATURAL_SEM.
+
+
+
+
+
+Module Type PE_REF_NATURAL_SEM (R : RED_LANG) (PERS : PE_RED_REF_SEM R).
+
+  Module ST := PERS.ST.
+  Export ST.
+  Import R.
+
+
+  Axiom dec_context_not_val : 
+      forall ec {k} v1 v0, dec_context ec k v0 <> in_val v1.
+
+  Axiom dec_term_value : 
+      forall {k} (v : value k), dec_term v k = in_val v.
+
+
+  Inductive dec : term -> forall {k1 k2}, context k1 k2 -> value k1 -> Prop :=
+
+  | dec_r    : forall t {t0 k1 k2} {c : context k1 k2} {r  v},
+                 dec_term t k2 = in_red r -> 
+                 contract r = Some t0 -> 
+                 dec t0 c v ->
+                 dec t c v
+  | dec_val  : forall t {k} {v : value k},
+               ~ dead_ckind k ->
+                 dec_term t k = in_val v ->
+                 dec t [.] v
+  | dec_v_t  : forall t ec {t0 ec0} {k1 k2} {c : context k1 k2} {v v0},
+                 dec_term t (k2+>ec) = in_val v -> 
+                 dec_context ec k2 v = in_term t0 ec0 -> 
+                 dec t0 (ec0=:c) v0 ->
+                 dec t (ec=:c) v0
+  | dec_red  : forall t ec {t0} {k1 k2} {c : context k1 k2} {v v0 r},
+                 dec_term t (k2+>ec) = in_val v ->
+                 dec_context ec k2 v = in_red r -> 
+                 contract r = Some t0 -> 
+                 dec t0 c v0 ->
+                 dec t (ec=:c) v0
+  | dec_rec  : forall t {t0 ec} {k1 k2} {c : context k1 k2} {v},
+                 dec_term t k2 = in_term t0 ec ->
+                 dec t0 (ec=:c) v ->
+                 dec t c v.
+
+
+  Inductive eval : term -> value init_ckind -> Prop :=
+  | e_intro : forall {t v}, dec t [.] v -> eval t v.
+
+End PE_REF_NATURAL_SEM.
+
+
+
+
+
+(*** Functors ***)
+
+
+Require Import Util.
+Require Export reduction_strategy.
+
+
+
+Module PreRefNaturalSem (R : RED_LANG) (RS : RED_REF_SEM R) 
+                                                <: PRE_REF_NATURAL_SEM R RS.
+
+  Module ST := RS.ST.
+  Export ST.
+  Import R.
+
+
+  Inductive dec : term -> forall {k1 k2}, context k1 k2 -> decomp k1 -> Prop :=
+
+  | d_dec  : forall t {k1 k2} (c : context k1 k2) {r},
+               dec_term t k2 = in_red r -> 
+               dec t c (d_red r c)
+  | d_v    : forall t {k1 k2} {c : context k1 k2} {v d},
+               dec_term t k2 = in_val v ->
+               decctx v c d ->
+               dec t c d
+  | d_term : forall t {t0 k1 k2} {c : context k1 k2} {ec d},
+               dec_term t k2 = in_term t0 ec ->
+               dec t0 (ec=:c) d ->
+               dec t c d
+
+  with decctx : forall {k2}, value k2 -> 
+                    forall {k1}, context k1 k2 -> decomp k1 -> Prop :=
+
+  | dc_end  : forall {k} (v : value k), 
+                ~ dead_ckind k ->
+                decctx v [.] (d_val v)
+  | dc_dec  : forall ec {k2} (v : value (k2+>ec)) {k1} (c : context k1 k2) {r},
+                dec_context ec k2 v = in_red r ->
+                decctx v (ec=:c) (d_red r c)
+  | dc_val  : forall {k2} {v0 : value k2} ec (v : value (k2+>ec)) 
+                     {k1} {c  : context k1 k2} {d},
+                dec_context ec k2 v = in_val v0 ->
+                decctx v0 c d ->
+                decctx v (ec=:c) d
+  | dc_term : forall ec {ec0 k2} (v : value (k2+>ec)) 
+                            {k1} {c : context k1 k2} {t d},
+                dec_context ec k2 v = in_term t ec0 ->
+                dec t (ec0=:c) d ->
+                decctx v (ec=:c) d.
+
+  Scheme dec_Ind    := Induction for dec Sort Prop
+    with decctx_Ind := Induction for decctx Sort Prop.
+
+
+  Inductive iter : forall {k}, decomp k -> value k -> Prop :=
+  | i_val : forall {k} (v : value k), 
+              iter (d_val v) v
+  | i_red : forall {k2} (r : redex k2) {t k1} {c : context k1 k2} {d v},
+              contract r = Some t -> 
+              dec t c d -> 
+              iter d v ->
+              iter (d_red r c) v.
+
+
+  Inductive eval : term -> value init_ckind -> Prop :=
+  | e_intro : forall {t d v}, dec t [.] d -> iter d v -> eval t v.
+
+End PreRefNaturalSem.
+
+
+
+
+Module StagedRefNaturalSem (R : RED_LANG) (RS : RED_REF_SEM R) 
+                                                <: STAGED_REF_NATURAL_SEM R RS.
+
+  Module ST := RS.ST.
+  Import R.
+  Export ST.
+
+
+  Inductive dec : term -> forall {k1 k2}, context k1 k2 -> value k1 -> Prop :=
+
+  | d_dec  : forall t {k1 k2} {c : context k1 k2} {r v},
+               dec_term t k2 = in_red r -> 
+               iter (d_red r c) v ->
+               dec t c v
+  | d_v    : forall t {k1 k2} {c : context k1 k2} {v v0},
+               dec_term t k2 = in_val v -> 
+               decctx v c v0 ->
+               dec t c v0
+  | d_many : forall t {t0 ec k1 k2} {c : context k1 k2} {v},
+               dec_term t k2 = in_term t0 ec -> 
+               dec t0 (ec=:c) v ->
+               dec t c v
+
+  with decctx : forall {k2}, value k2 -> 
+                    forall {k1}, context k1 k2 -> value k1 -> Prop :=
+
+  | dc_end  : forall {k} {v v0 : value k},
+                ~ dead_ckind k ->
+                iter (d_val v) v0 ->
+                decctx v [.] v0
+  | dc_dec  : forall ec {k2} (v : value (k2+>ec)) {k1} {c : context k1 k2} {r v0},
+                dec_context ec k2 v = in_red r -> 
+                iter (d_red r c) v0 ->
+                decctx v (ec=:c) v0
+  | dc_val  : forall ec {k2} (v : value (k2+>ec)) {v0 k1} {c : context k1 k2} {v1},
+                dec_context ec k2 v = in_val v0 -> 
+                decctx v0 c v1 ->
+                decctx v (ec=:c) v1
+  | dc_term : forall ec {k2} (v : value (k2+>ec)) {t ec0 k1} {c : context k1 k2} {v0},
+                dec_context ec k2 v = in_term t ec0 -> 
+                dec t (ec0=:c) v0 ->
+                decctx v (ec=:c) v0
+
+  with iter : forall {k}, decomp k -> value k -> Prop :=
+
+  | i_val : forall {k} (v : value k), 
+              iter (d_val v) v
+  | i_red : forall {k2} (r : redex k2) {k1} {c : context k1 k2} {t v},
+              contract r = Some t -> 
+              dec t c v -> 
+              iter (d_red r c) v.
+
+  Scheme dec_Ind    := Induction for dec    Sort Prop
+    with decctx_Ind := Induction for decctx Sort Prop
+    with iter_Ind   := Induction for iter   Sort Prop.
+
+
+  Inductive eval : term -> value init_ckind -> Prop :=
+  | e_intro : forall {t v}, dec t [.] v -> eval t v.
+
+End StagedRefNaturalSem.
+
+
+
+
+Module RefNaturalSem (R : RED_LANG) (RS : RED_REF_SEM R)
+                                              <: REF_NATURAL_SEM R RS.
+
+  Module ST := RS.ST.
+  Export ST.
+  Import R.
+
+
+  Inductive dec : term -> forall {k1 k2}, context k1 k2 -> value k1 -> Prop :=
+
+  | d_d_r  : forall t {t0 k1 k2} {c : context k1 k2} {r : redex k2} {v},
+               dec_term t k2 = in_red r -> 
+               contract r = Some t0 -> 
+               dec t0 c v ->
+               dec t c v
+  | d_v    : forall t {k1 k2} {c : context k1 k2} {v v0},
+               dec_term t k2 = in_val v -> 
+               decctx v c v0 ->
+               dec t c v0
+  | d_term : forall t {t0 ec k1 k2} {c : context k1 k2} {v},
+               dec_term t k2 = in_term t0 ec -> 
+               dec t0 (ec=:c) v ->
+               dec t c v
+
+  with decctx : forall {k2}, value k2 -> 
+                    forall {k1}, context k1 k2 -> value k1 -> Prop :=
+
+  | dc_end : forall {k} (v : value k), 
+               ~ dead_ckind k ->
+               decctx v [.] v
+  | dc_red : forall ec {k2} (v : value (k2+>ec)) {k1} {c : context k1 k2} {r t v0},
+               dec_context ec k2 v = in_red r -> 
+               contract r = Some t -> 
+               dec t c v0 ->
+               decctx v (ec=:c) v0
+  | dc_rec : forall ec {k2} (v : value (k2+>ec)) {k1} {c : context k1 k2} {v0 v1},
+               dec_context ec k2 v = in_val v0 -> 
+               decctx v0 c v1 ->
+               decctx v (ec=:c) v1
+  | dc_trm : forall ec {k2} (v : value (k2+>ec)) {k1} {c : context k1 k2} {t ec0 v0},
+               dec_context ec k2 v = in_term t ec0 -> 
+               dec t (ec0=:c) v0 ->
+               decctx v (ec=:c) v0.
+
+  Scheme dec_Ind    := Induction for dec    Sort Prop
+    with decctx_Ind := Induction for decctx Sort Prop.
+
+
+  Inductive eval : term -> value init_ckind -> Prop :=
+  | e_intro : forall {t v}, dec t [.] v -> eval t v.
+
+End RefNaturalSem.
+
+
+
+
+Module PE_RefNaturalSem (R : RED_LANG) (PERS : PE_RED_REF_SEM R)
+                                                  <: PE_REF_NATURAL_SEM R PERS.
+
+  Module ST := PERS.ST.
+  Export ST.
+  Import R.
+
+
+  Axiom dec_context_not_val : 
+      forall ec {k} v1 v0, dec_context ec k v0 <> in_val v1.
+
+  Axiom dec_term_value : 
+      forall {k} (v : value k), dec_term v k = in_val v.
+
+
+  Inductive dec : term -> forall {k1 k2}, context k1 k2 -> value k1 -> Prop :=
+
+  | dec_r    : forall t {t0 k1 k2} {c : context k1 k2} {r  v},
+                 dec_term t k2 = in_red r -> 
+                 contract r = Some t0 -> 
+                 dec t0 c v ->
+                 dec t c v
+  | dec_val  : forall t {k} {v : value k},
+               ~ dead_ckind k ->
+                 dec_term t k = in_val v ->
+                 dec t [.] v
+  | dec_v_t  : forall t ec {t0 ec0} {k1 k2} {c : context k1 k2} {v v0},
+                 dec_term t (k2+>ec) = in_val v -> 
+                 dec_context ec k2 v = in_term t0 ec0 -> 
+                 dec t0 (ec0=:c) v0 ->
+                 dec t (ec=:c) v0
+  | dec_red  : forall t ec {t0} {k1 k2} {c : context k1 k2} {v v0 r},
+                 dec_term t (k2+>ec) = in_val v ->
+                 dec_context ec k2 v = in_red r -> 
+                 contract r = Some t0 -> 
+                 dec t0 c v0 ->
+                 dec t (ec=:c) v0
+  | dec_rec  : forall t {t0 ec} {k1 k2} {c : context k1 k2} {v},
+                 dec_term t k2 = in_term t0 ec ->
+                 dec t0 (ec=:c) v ->
+                 dec t c v.
+
+
+  Inductive eval : term -> value init_ckind -> Prop :=
+  | e_intro : forall {t v}, dec t [.] v -> eval t v.
+
+End PE_RefNaturalSem.
+
+
